wip: introduce a new symbol UNKNOWN to X^+.
This solves several issues:
- We don't have to invent default symbols for the sigma-lift, it is
  simply `inl UNKNOWN`.
- It simplifies the lemma contains_translate_tau2, where we now only
  have in the premise that each symbol of the mapped encoding can be
  mapped back to sigma.
- We don't have to give a default symbol for each tape
- Liftings, for example from `bool` to `bool+X`, where previously not
  possible. We couldn't lift `MatchNat` from `bool^+` to `(bool+X)`,
  because whatever default symbol we choose (i.e `true` or `false`), it
  is in the encoding of the output.

TM/Code/CodeTM.v
@@ -55,14 +55,15 @@ End IsRight.
 (** Type for start and stop symbols, isomorphic to [bool] *)
 
 Inductive boundary : Type :=
-| START : boundary
-| STOP  : boundary.
+| START   : boundary
+| STOP    : boundary
+| UNKNOWN : boundary.
 
 Instance boundary_eq : eq_dec boundary.
 Proof. unfold dec. decide equality. Defined.
 
 Instance boundary_fin : finTypeC (EqType boundary).
-Proof. split with (enum := [START; STOP]). cbn. intros []; cbn; reflexivity. Defined.
+Proof. split with (enum := [START; STOP; UNKNOWN]). cbn. intros []; cbn; reflexivity. Defined.
 
 
 Notation "sig '^+'" := (FinType(EqType(boundary + sig))) (at level 0) : type_scope.
